feat(BKS & BKSA)!: Smithy Model for HV-2 (#1350)
BREAKING CHANGE: Branch Key Store Admin has the following breaking changes for MRK support:
- `KmsSymmetricKeyArn` has dropped the MRK option entirely

AwsCryptographicMaterialProviders/runtimes/java/src/examples/java/software/amazon/cryptography/example/hierarchy/mutations/MutationsProvider.java
@@ -20,6 +20,7 @@ import software.amazon.cryptography.keystoreadmin.model.InitializeMutationInput;
 import software.amazon.cryptography.keystoreadmin.model.InitializeMutationOutput;
 import software.amazon.cryptography.keystoreadmin.model.KeyManagementStrategy;
 import software.amazon.cryptography.keystoreadmin.model.KmsSymmetricEncryption;
+import software.amazon.cryptography.keystoreadmin.model.KmsSymmetricKeyArn;
 import software.amazon.cryptography.keystoreadmin.model.MutatedBranchKeyItem;
 import software.amazon.cryptography.keystoreadmin.model.MutationToken;
 import software.amazon.cryptography.keystoreadmin.model.Mutations;
