AwsCryptographicMaterialProviders/runtimes/java/src/main/smithy-generated/software/amazon/cryptography/keystoreadmin/model/MutableBranchKeyContext.java
@@ -1,0 +1,165 @@
+// Copyright Amazon.com Inc. or its affiliates. All Rights Reserved.
+// SPDX-License-Identifier: Apache-2.0
+// Do not modify this file. This file is machine generated, and any changes to it will be overwritten.
+package software.amazon.cryptography.keystoreadmin.model;
+
+import java.util.Map;
+import java.util.Objects;
+import software.amazon.cryptography.keystore.model.HierarchyVersion;
+
+/**
+ *
+ * Define the Mutable Context of a Branch Key.
+ * As of v1.9.0, the Mutable Context are:
+ * - The KmsArn protecting the Branch Key
+ * - The encryption context of a Branch Key
+ */
+public class MutableBranchKeyContext {
+
+  /**
+   * The KmsArn protecting the Branch Key.
+   */
+  private final String KmsArn;
+
+  /**
+   * The Encryption Context authenticated with this Branch Key.
+   */
+  private final Map<String, String> EncryptionContext;
+
+  /**
+   * The 'hierarchy-version' of the Branch Key.
+   */
+  private final HierarchyVersion HierarchyVersion;
+
+  protected MutableBranchKeyContext(BuilderImpl builder) {
+    this.KmsArn = builder.KmsArn();
+    this.EncryptionContext = builder.EncryptionContext();
+    this.HierarchyVersion = builder.HierarchyVersion();
+  }
+
+  /**
+   * @return The KmsArn protecting the Branch Key.
+   */
+  public String KmsArn() {
+    return this.KmsArn;
+  }
+
+  /**
+   * @return The Encryption Context authenticated with this Branch Key.
+   */
+  public Map<String, String> EncryptionContext() {
+    return this.EncryptionContext;
+  }
+
+  /**
+   * @return The 'hierarchy-version' of the Branch Key.
+   */
+  public HierarchyVersion HierarchyVersion() {
+    return this.HierarchyVersion;
+  }
+
+  public Builder toBuilder() {
+    return new BuilderImpl(this);
+  }
+
+  public static Builder builder() {
+    return new BuilderImpl();
+  }
+
+  public interface Builder {
+    /**
+     * @param KmsArn The KmsArn protecting the Branch Key.
+     */
+    Builder KmsArn(String KmsArn);
+
+    /**
+     * @return The KmsArn protecting the Branch Key.
+     */
+    String KmsArn();
+
+    /**
+     * @param EncryptionContext The Encryption Context authenticated with this Branch Key.
+     */
+    Builder EncryptionContext(Map<String, String> EncryptionContext);
+
+    /**
+     * @return The Encryption Context authenticated with this Branch Key.
+     */
+    Map<String, String> EncryptionContext();
+
+    /**
+     * @param HierarchyVersion The 'hierarchy-version' of the Branch Key.
+     */
+    Builder HierarchyVersion(HierarchyVersion HierarchyVersion);
+
+    /**
+     * @return The 'hierarchy-version' of the Branch Key.
+     */
+    HierarchyVersion HierarchyVersion();
+
+    MutableBranchKeyContext build();
+  }
+
+  static class BuilderImpl implements Builder {
+
+    protected String KmsArn;
+
+    protected Map<String, String> EncryptionContext;
+
+    protected HierarchyVersion HierarchyVersion;
+
+    protected BuilderImpl() {}
+
+    protected BuilderImpl(MutableBranchKeyContext model) {
+      this.KmsArn = model.KmsArn();
+      this.EncryptionContext = model.EncryptionContext();
+      this.HierarchyVersion = model.HierarchyVersion();
+    }
+
+    public Builder KmsArn(String KmsArn) {
+      this.KmsArn = KmsArn;
+      return this;
+    }
+
+    public String KmsArn() {
+      return this.KmsArn;
+    }
+
+    public Builder EncryptionContext(Map<String, String> EncryptionContext) {
+      this.EncryptionContext = EncryptionContext;
+      return this;
+    }
+
+    public Map<String, String> EncryptionContext() {
+      return this.EncryptionContext;
+    }
+
+    public Builder HierarchyVersion(HierarchyVersion HierarchyVersion) {
+      this.HierarchyVersion = HierarchyVersion;
+      return this;
+    }
+
+    public HierarchyVersion HierarchyVersion() {
+      return this.HierarchyVersion;
+    }
+
+    public MutableBranchKeyContext build() {
+      if (Objects.isNull(this.KmsArn())) {
+        throw new IllegalArgumentException(
+          "Missing value for required field `KmsArn`"
+        );
+      }
+      if (Objects.isNull(this.EncryptionContext())) {
+        throw new IllegalArgumentException(
+          "Missing value for required field `EncryptionContext`"
+        );
+      }
+      if (Objects.isNull(this.HierarchyVersion())) {
+        throw new IllegalArgumentException(
+          "Missing value for required field `HierarchyVersion`"
+        );
+      }
+      return new MutableBranchKeyContext(this);
+    }
+  }
+}
