AwsCryptographicMaterialProviders/runtimes/java/src/testExamples/java/software/amazon/cryptography/example/hierarchy/mutations/MutationKmsAccessOriginalInFlightTest.java
@@ -29,6 +29,7 @@ import software.amazon.cryptography.keystoreadmin.model.InitializeMutationInput;
 import software.amazon.cryptography.keystoreadmin.model.InitializeMutationOutput;
 import software.amazon.cryptography.keystoreadmin.model.KeyManagementStrategy;
 import software.amazon.cryptography.keystoreadmin.model.KeyStoreAdminException;
+import software.amazon.cryptography.keystoreadmin.model.KmsSymmetricKeyArn;
 import software.amazon.cryptography.keystoreadmin.model.MutationFromException;
 import software.amazon.cryptography.keystoreadmin.model.MutationToException;
 import software.amazon.cryptography.keystoreadmin.model.MutationToken;
